theories/program_logic/lifting.v
@@ -1,3 +1,74 @@
+Inductive natlist : Type :=
+  | nil : natlist
+  | cons : nat -> natlist -> natlist.
+
+Fixpoint app (l1 l2 : natlist) : natlist :=
+  match l1 with nil => l2 | cons x l1 => cons x (app l1 l2) end.
+
+Fixpoint rev (l : natlist) : natlist :=
+  match l with nil => nil | cons x l => app (rev l) (cons x nil) end.
+
+Inductive palindrome : natlist -> Prop :=
+  | nilp : palindrome nil
+  | consp : forall x xs, palindrome xs -> palindrome (cons x (app xs (cons x nil))).
+
+Lemma consrev l x : cons x (rev l) = rev (app l (cons x nil)).
+Proof.
+  induction l; simpl; auto.
+  rewrite <-IHl; simpl. auto.
+Qed.
+
+Lemma prev l : palindrome l -> rev l = l.
+Proof.
+  induction 1; auto.
+  simpl.
+  rewrite<-consrev.
+  rewrite IHpalindrome.
+  reflexivity.
+Qed.
+
+Definition id := nat.
+
+Inductive expr :=
+| EVar (x : id) : expr
+| ENat (n : nat) : expr
+| EBool (b : bool) : expr
+| ELet (x : id) (e1 e2 : expr) : expr
+| EIf (e1 e2 e3 : expr) : expr.
+
+Inductive val :=
+  | VNat : nat -> val
+  | VBool : bool -> val.
+
+Inductive env :=
+  | env_nil
+  | env_snoc (E : env) (x : id) (v : val) : env.
+
+Fixpoint env_lookup (x : id) (E : env) : option val := None.
+
+Fixpoint interp (E : env) (e : expr) : option val :=
+  match e with
+  | EVar x => env_lookup x E
+  | ENat n => Some (VNat n)
+  | EBool b => Some (VBool b)
+  | ELet x e1 e2 =>
+     match interp E e1 with
+     | Some v1 => interp (env_snoc E x v1) e2
+     | None => None
+     end
+  | EIf e1 e2 e3 =>
+    match interp E e1 with
+    | Some (VBool true) => interp E e2
+    | Some (VBool false) => interp E e3
+    | _ => None
+    end
+  end.
+
+Inductive big_step : expr -> val -> Prop := .
+
+
+Lemma interp_big_step e v : interp env_nil e = Some v <-> big_step e v.
+
 From iris.proofmode Require Import tactics.
 From diris.program_logic Require Export weakestpre.
 Set Default Proof Using "Type".
@@ -10,7 +81,6 @@ Implicit Types e : expr Λ.
 Implicit Types σ : state Λ.
 Implicit Types P Q : iProp Σ.
 Implicit Types Φ : val Λ → iProp Σ.
-
 Hint Resolve reducible_no_obs_reducible : core.
 
 Lemma wp_lift_step_fupd s E Φ e1 :
@@ -18,7 +88,7 @@ Lemma wp_lift_step_fupd s E Φ e1 :
   (∀ ζ σ1 κ κs es tid,
      ⌜ tid_get s tid ∧ es !! tid = Some e1 ⌝ -∗
      state_interp ζ σ1 (κ ++ κs) es ={E,∅}=∗
-       ⌜ state_valid ζ σ1 s e1 ⌝ ∧
+       ⌜ reducible e1 σ1 ∨ stuck_valid ζ σ1 s e1 ⌝ ∧
        ∀ e2 σ2 efs,
          ⌜ prim_step e1 σ1 κ e2 σ2 efs ⌝ ={∅,∅,E}▷=∗
          ∃ ζ', state_interp ζ' σ2 κs (<[tid:=e2]> es ++ efs) ∗
@@ -58,12 +128,16 @@ Proof.
 Qed. *)
 
 
-(* state_valid : abstract_state → state Λ → A → expr Λ → Prop; *)
-Lemma wp_lift_pure_step_no_fork `{!Inhabited (state Λ)} s E E' Φ e1 :
+(* stuck_valid : abstract_state → state Λ → A → expr Λ → Prop; *)
+Lemma wp_lift_pure_step_no_fork s E E' Φ e1 :
   to_val e1 = None →
-  (∀ ζ σ1, state_valid ζ σ1 s e1) →
-  (∀ κ κs σ1 e2 σ2 efs es i  ζ, tid_get s i → prim_step e1 σ1 κ e2 σ2 efs → κ = [] ∧ σ2 = σ1 ∧ efs = [] ∧
-    (state_interp ζ σ1 κs (<[i:=e1]> es) ⊢ state_interp ζ σ2 κs (<[i:=e2]> es))) →
+  (∀ ζ σ1, reducible e1 σ1 ∨ stuck_valid ζ σ1 s e1) →
+  (∀ κ σ1 e2 σ2 efs ,
+    prim_step e1 σ1 κ e2 σ2 efs →
+    κ = [] ∧ σ2 = σ1 ∧ efs = [] ∧
+    (∀ κs es tid ζ,
+      tid_get s tid →
+      state_interp ζ σ1 κs (<[tid:=e1]> es) ⊢ state_interp ζ σ2 κs (<[tid:=e2]> es))) →
   (|={E,E'}▷=> ∀ κ e2 efs σ, ⌜prim_step e1 σ κ e2 σ efs⌝ → WP e2 @ s; E {{ Φ }})
   ⊢ WP e1 @ s; E {{ Φ }}.
 Proof.
@@ -75,7 +149,7 @@ Proof.
   iModIntro.
   iSplit; first done.
   iIntros (e2 σ2 efs primst).
-  destruct (Hstep κ κs σ1 e2 σ2 efs es tid ζ) as (-> & <- & -> & Hsi);[done..|].
+  destruct (Hstep κ σ1 e2 σ2 efs) as (-> & <- & -> & Hsi);[done..|].
   iMod "Hclose" as "_".
   iExists ζ. simpl.
   replace (state_interp ζ σ2 κs es) with (state_interp ζ σ2 κs (<[tid:=e1]> es)) by
@@ -117,22 +191,22 @@ Qed. *)
 
 (* Atomic steps don't need any mask-changing business here, one can
    use the generic lemmas here. *)
-Lemma wp_lift_atomic_step_fupd {s i E1 E2 Φ} e1 :
-  tid_get s i →
+Lemma wp_lift_atomic_step_fupd {s E1 E2 Φ} e1 :
   to_val e1 = None →
-  (∀ ζ σ1 κ κs es, state_interp ζ σ1 (κ ++ κs) es ={E1}=∗
-    ⌜state_valid ζ σ1 s e1⌝ ∗
+  (∀ ζ σ1 κ κs es tid,
+    ⌜ tid_get s tid ∧ es !! tid = Some e1 ⌝ -∗
+    state_interp ζ σ1 (κ ++ κs) es ={E1}=∗
+    ⌜ reducible e1 σ1 ∨ stuck_valid ζ σ1 s e1 ⌝ ∗
     ∀ e2 σ2 efs, ⌜prim_step e1 σ1 κ e2 σ2 efs⌝ ={E1,E2}▷=∗
-      ∃ ζ', state_interp ζ' σ2 κs ((<[i := e2]> es) ++ efs) ∗
+      ∃ ζ', state_interp ζ' σ2 κs ((<[tid := e2]> es) ++ efs) ∗
       from_option Φ False (to_val e2) ∗
       [∗ list] i ↦ ef ∈ efs, WP ef @ (tid_set (i + length es) s); ⊤ {{ fork_post (i + length es) }})
   ⊢ WP e1 @ s; E1 {{ Φ }}.
 Proof.
-  iIntros (tidg1 ?) "H".
+  iIntros (?) "H".
   iApply wp_lift_step_fupd; first done.
-  iIntros (ζ σ1 κ κs es tid [tidg2 tidh]) "Hsi".
-  pose proof (tid_func _ _ _ tidg1 tidg2). subst.
-  iMod ("H" with "Hsi") as "[$ H]".
+  iIntros (ζ σ1 κ κs es tid [tidg tidh]) "Hsi".
+  iMod ("H" with "[//] Hsi") as "[$ H]".
   iMod (fupd_intro_mask' E1 ∅) as "Hclose"; first by apply empty_subseteq.
   iModIntro. iIntros (e2 σ2 efs Hps).
   iMod "Hclose" as "_".
@@ -161,49 +235,36 @@ Proof.
   by iApply "H".
 Qed. *)
 
-(*
-Lemma wp_lift_pure_step_no_fork `{!Inhabited (state Λ)} s E E' Φ e1 :
-  to_val e1 = None →
-  (∀ ζ σ1, state_valid ζ σ1 s e1) →
-  (∀ κ κs σ1 e2 σ2 efs es i  ζ, tid_get s i → prim_step e1 σ1 κ e2 σ2 efs → κ = [] ∧ σ2 = σ1 ∧ efs = [] ∧
-    (state_interp ζ σ1 κs (<[i:=e1]> es) ⊢ state_interp ζ σ2 κs (<[i:=e2]> es))) →
-  (|={E,E'}▷=> ∀ κ e2 efs σ, ⌜prim_step e1 σ κ e2 σ efs⌝ → WP e2 @ s; E {{ Φ }})
-  ⊢ WP e1 @ s; E {{ Φ }}.
-Proof.
-
-Lemma wp_lift_pure_det_step_no_fork `{!Inhabited (state Λ)} {s i E E' Φ} e1 e2 :
-  (∀ σ1, if s is NotStuck then reducible e1 σ1 ∨ waiting e1 σ1 else to_val e1 = None) →
-  (∀ σ1 κ e2' σ2 efs', prim_step e1 σ1 κ e2' σ2 efs' →
-    κ = [] ∧ σ2 = σ1 ∧ e2' = e2 ∧ efs' = []) →
-  (|={E,E'}▷=> WP e2 @ (s,i); E {{ Φ }}) ⊢ WP e1 @ (s,i); E {{ Φ }}.
-Proof.
-  *)
 
 Lemma wp_lift_pure_det_step_no_fork `{!Inhabited (state Λ)} {s E E' Φ} e1 e2 :
   to_val e1 = None →
-  (∀ ζ σ1, state_valid ζ σ1 s e1) →
-  (∀ κ σ1 e2' σ2 efs',  prim_step e1 σ1 κ e2' σ2 efs' →
+  (∀ ζ σ1, reducible e1 σ1 ∨ stuck_valid ζ σ1 s e1) →
+  (∀ κ σ1 e2' σ2 efs',
+    prim_step e1 σ1 κ e2' σ2 efs' →
     κ = [] ∧ σ2 = σ1 ∧ e2' = e2 ∧ efs' = [] ∧
-    (∀ κs es i ζ, tid_get s i → state_interp ζ σ1 κs (<[i:=e1]> es) ⊢ state_interp ζ σ2 κs (<[i:=e2]> es))) →
+    (∀ κs es tid ζ,
+      tid_get s tid →
+      state_interp ζ σ1 κs (<[tid:=e1]> es) ⊢ state_interp ζ σ2 κs (<[tid:=e2]> es))) →
   (|={E,E'}▷=> WP e2 @ s; E {{ Φ }}) ⊢ WP e1 @ s; E {{ Φ }}.
 Proof.
   iIntros (?? Hpuredet) "H". iApply (wp_lift_pure_step_no_fork s E E'); try done.
   { intros. edestruct Hpuredet as (? & ? & ? & ? & ?); eauto. subst. eauto. }
   iApply (step_fupd_wand with "H"); iIntros "H".
   iIntros (κ e' efs' σ Hps).
-  pose proof (tid_exists s) as [i Htid].
   eapply Hpuredet in Hps as (? & ? & -> & ?). done.
 Qed.
 
-Lemma wp_pure_step_fupd `{!Inhabited (state Λ)} s i E E' e1 e2 φ n Φ :
+Lemma wp_pure_step_fupd `{!Inhabited (state Λ)} s E E' e1 e2 φ n Φ :
   PureExec φ n e1 e2 →
   φ →
-  (|={E,E'}▷=>^n WP e2 @ (s,i); E {{ Φ }}) ⊢ WP e1 @ (s,i); E {{ Φ }}.
+  (|={E,E'}▷=>^n WP e2 @ s; E {{ Φ }}) ⊢ WP e1 @ s; E {{ Φ }}.
 Proof.
   iIntros (Hexec Hφ) "Hwp". specialize (Hexec Hφ).
   iInduction Hexec as [e|n e1 e2 e3 [Hsafe ?]] "IH"; simpl; first done.
-  iApply wp_lift_pure_det_step_no_fork.
-  - intros σ. specialize (Hsafe σ). destruct s; eauto using reducible_not_val.
+  iApply wp_lift_pure_det_step_no_fork;
+    eauto using reducible_no_obs_reducible, reducible_not_val.
+  -
+  - eauto.
   - done.
   - by iApply (step_fupd_wand with "Hwp").
 Qed.
