theories/bi/weakestpre.v
@@ -1,7 +1,6 @@
 From stdpp Require Export coPset.
 From iris.bi Require Import interface derived_connectives.
-From diris.program_logic Require Import language.
-
+From iris.program_logic Require Import language.
 
 Inductive stuckness := NotStuck | MaybeStuck.
 
