theories/program_logic/order.v
@@ -1,0 +1,42 @@
+From iris.proofmode Require Import base tactics classes.
+
+Inductive comparison := LT | GT | EQ.
+
+Fixpoint cmp a b :=
+    match a,b with
+    | true::a, true::b | false::a, false::b => cmp a b
+    | [],[] => EQ
+    | false::_, _ | _,true::_ => LT
+    | true::_, _ | _,false::_ => GT
+    end.
+
+Definition inv_comparison a :=
+    match a with
+    LT => GT | GT => LT | EQ => EQ
+    end.
+
+Lemma cmp_inv a b : cmp a b = inv_comparison (cmp b a).
+Proof.
+    revert b; induction a; intros; destruct b; destr_bool; auto.
+Qed.
+
+Lemma cmp_eq a b : cmp a b = EQ <-> a = b.
+Proof.
+    revert b; induction a; intros; destruct b; destr_bool;
+    rewrite ?IHa; split; intros; simplify_eq; reflexivity.
+Qed.
+
+Lemma cmp_app x a b : cmp (x ++ a) (x ++ b) = cmp a b.
+Proof.
+    induction x; simpl; destr_bool.
+Qed.
+
+Definition below x := x ++ [false].
+Definition above x := x ++ [true].
+
+Lemma below_cmp x : cmp (below x) x = LT.
+Proof.
+    replace (cmp (below x) x) with (cmp (x ++ [false]) (x ++ [])).
+    { rewrite cmp_app. reflexivity. }
+    f_equal. apply app_nil_r.
+Qed.
